Data-dependent loop primitive defined.
Also
- some trivial lemmas about ddepR; and
- statement of correctness for the desired loop transformation
  captured.

Still assuming that the δ mapping will preserve domains:

  [0,N) <-> [0,N)

in fact.

hol/datadepsScript.sml
@@ -1,55 +1,80 @@
 open HolKernel Parse boolLib bossLib;
+open primitivesTheory
+open lcsymtacs
 
 val _ = new_theory "datadeps";
 
 val eval_def = Define`
-  eval A body Wf Rs i =
-    update A (Wf i) (body (MAP (λf. f i) Rs))
+  eval Wf Rs vf i A =
+    update A (Wf i) (vf i (MAP (λf. vsub A (f i)) Rs))
 `;
 
+val example_t =
+  ``FOR (0,N)
+      (eval (vsub (f : num mvector))
+            [(λi. i + 1); vsub (h : num mvector)]
+            (λi rds. EL 0 rds + EL 1 rds + 1))``;
+
+val computation =
+    EVAL ``let N = 5 in
+           let f = ((λi. EL i [4;3;2;1;0]), 5) in
+           let h = ((λi. EL i [0;1;1;2;3]), 5) in
+             ^example_t ((λi. EL i [0;0;0;0;0;0]), 6)``
+
+
 (* C original:
+int N = 5;
+int A[6] = {0};
+int f[5] = {4,3,2,1,0};
+int h[5] = {0,1,1,2,3};
+
 for (int i= 0; i < N; i++)
   A[f[i]] = A[i+1] + A [h[i]];
 
-for (int j=lo; j < M; j++)
-  A[f[
 
 *)
 
-val eg1_def = Define`
-  FOR (0,100)
-      (λi A.
-        eval A (λris. A ' (EL 0 ris) + A ' (EL 1 ris))
-             (λi. f ' i)
-             [(λi. g ' i); (λi. h ' i)]
-             i)
-`;
+val _ = overload_on("@@", ``λl x. MAP (combin$C I x) l``)
+val _ = set_fixity "@@" (Infixl 2000)
 
-
-FOR (lo,hi) (λi A. eval f wi ris i)
-
-val ddepR = Define`
+val ddepR_def = Define`
   ddepR wf rfs i0 i ⇔
     i0 < i ∧ (wf i0 = wf i ∨
-              MEM (wf i0) (rfs i) ∨
-              MEM (wf i) (rfs i0))
+              MEM (wf i0) (rfs @@ i) ∨
+              MEM (wf i) (rfs @@ i0))
 `;
 
+val ddepR_irreflexive = store_thm(
+  "ddepR_irreflexive",
+  ``∀i. ¬ddepR wf rfs i i``,
+  rw[ddepR_def]);
+val _ = export_rewrites ["ddepR_irreflexive"]
 
-domain1 = domain2 ∧ wi' = wi o dinv ∧ ris' = ris' o dinv ∧
-BIJ dinv (count N) (count N)
+val ddepR_TC_LT = store_thm(
+  "ddepR_TC_LT",
+  ``∀i j. (ddepR wf rfs)⁺ i j ⇒ i < j``,
+  ho_match_mp_tac relationTheory.TC_INDUCT >>
+  rw[ddepR_def] >> decide_tac);
+
+val ddepR_acyclic = store_thm(
+  "ddepR_acyclic",
+  ``∀i. ¬(ddepR wf rfs)⁺ i i``,
+  rpt strip_tac >> imp_res_tac ddepR_TC_LT >> fs[]);
+val _ = export_rewrites ["ddepR_acyclic"]
+
+(*
+val correctness = store_thm(
+  "correctness",
+  ``(∀i0 i. ddepR wf rfs i0 i ==> δ i0 < δ i) ∧
+    BIJ δ (count N) (count N) ∧
+    γ = LINV δ (count N)
+  ==>
+    FOR (0,N) (eval wf rfs body) =
+    FOR (0,N) (eval (wf o γ)
+                    (MAP (λf. f o γ) rds)
+                    body)``
 
 
-(ddepR wf rfs i0 i ==> δ i0 < δ i (in domain2))
-∧
- BIJ δ domain1 domain2
 
-==>
-
-FOR i ∈ domain1 { update A wf rfs i } =
-FOR j ∈ domain2 { update A (wf o δ⁻¹) (rfs o δ⁻¹) j }
-
-
-
-
+*)
 val _ = export_theory();
